steps

compiler/scheme/scheme_semanticsScript.sml
@@ -3,6 +3,7 @@
 *)
 open preamble;
 open prim_recTheory;
+open mesonLib;
 open mlstringTheory;
 open scheme_astTheory;
 
@@ -26,32 +27,29 @@ End
 
 Definition strict_def:
   strict (Prim SAdd) xs = sadd xs 0 ∧
-  strict (Prim SMul) xs = smul xs 1 ∧
-  strict _ _ = Wrong "Not supported"
+  strict (Prim SMul) xs = smul xs 1
 End
 
 Definition semantics_def:
   semantics (Val v) = v ∧
-  semantics (Apply fn args) = strict (semantics fn) (MAP semantics args) ∧
-  semantics (Print _) = Wrong "Not supported"
+  semantics (Apply fn args) = strict (semantics fn) (MAP semantics args)
 Termination
   WF_REL_TAC ‘measure exp_size’
 End
 
 Definition return_def:
-  return ([], v) = ([], Val v) ∧
-  return (ApplyK NONE [] :: ks, v) = (ks, Val $ strict v []) ∧
-  return (ApplyK NONE (e::es) :: ks, v) = (ApplyK (SOME (v, [])) es :: ks, e) ∧
-  return (ApplyK (SOME (vfn, vargs)) [] :: ks, v) =
+  return [] v = ([], Val v) ∧
+  return (ApplyK NONE [] :: ks) v = (ks, Val $ strict v []) ∧
+  return (ApplyK NONE (e::es) :: ks) v = (ApplyK (SOME (v, [])) es :: ks, e) ∧
+  return (ApplyK (SOME (vfn, vargs)) [] :: ks) v =
     (ks, Val $ strict vfn (REVERSE $ v::vargs)) ∧
-  return (ApplyK (SOME (vfn, vargs)) (e::es) :: ks, v) =
+  return (ApplyK (SOME (vfn, vargs)) (e::es) :: ks) v =
     (ApplyK (SOME (vfn, v::vargs)) es ::ks, e)
 End
 
 Definition step_def:
-  step (ks, Val v) = return (ks, v) ∧
-  step (ks, Apply fn args) = (ApplyK NONE args :: ks, fn) ∧
-  step (_, Print _) = ([], Val $ Wrong "Not supported")
+  step ks (Val v) = return ks v ∧
+  step ks (Apply fn args) = (ApplyK NONE args :: ks, fn)
 End
 
 Definition big_step_def:
@@ -61,10 +59,68 @@ Definition big_step_def:
     else Wrong "Diverged"
 End
 
+Definition steps_def:
+  steps _ [] (Val v) = ([], Val v) ∧
+  steps (n:num) ks e = if n > 0
+    then let (ks', e') = (step ks e) in (steps (n - 1) ks' e')
+    else (ks, e)
+End
+
+Theorem steps_return:
+  ∀ e v n ks . steps n [] e = ([], Val v) ⇒ steps n ks e = return ks v
+Proof
+  Induct_on ‘ks’
+  Induct_on ‘l’
+  Induct_on ‘n’
+  fs[return_def]
+  fs[steps_def]
+  rw[steps_def]
+  rw[step_def]
+  rw[return_def]
+  rw[]
+  simp[steps_def]
+  ‘return ks' v'' = steps n'' ks' (Val v'')’ by rw[]
+  pop_assum(SUBST1_TAC o SYM o SPEC ``0:num`` o SPEC ``SNum 0``)
+  gs[]
+  first_x_assum $ qspecl_then [‘SNum 0’,‘0’] SUBST1_TAC
+  last_x_assum $ assume_tac o SRULE [Once EQ_SYM_EQ]
+  qexists_tac ‘n’
+  qexists_tac ‘n + 1’
+  Cases_on ‘o'’
+  Cases_on ‘v’
+  Cases_on ‘v'’
+  Cases_on ‘l’
+  Cases_on ‘ks’
+  Cases_on ‘n - 1 > 0’
+  MESON_TAC[steps_def]
+
 Theorem big_small_equiv:
-  ∀ e . ∃ n . big_step n ([], e) = semantics e
+  ∀ e v . semantics e = v ⇒ ∃ n . steps n ([], e) = ([], Val v)
 Proof
   rw[]
+  Induct
+  simp[]
+  fs[]
+  Induct_on ‘l’
+  Induct_on ‘e’
+  asm_simp_tac bool_ss []
+  SUBST1_TAC(ASSUME “return ks (SNum 0) = steps 0 ks (Val (SNum 0))”)
+  fs[steps_def, step_def, semantics_def,
+    return_def, strict_def, sadd_def, smul_def]
+  DISCH_TAC
+  rw[steps_def, step_def, semantics_def,
+    return_def, strict_def, sadd_def, smul_def]
+  metis_tac[steps_def, step_def, semantics_def,
+    return_def, strict_def, sadd_def, smul_def]
+  qexists_tac ‘n’
+  Cases_on ‘e’
+  Cases_on ‘p’
+  Cases_on ‘v’
+  Cases_on ‘h’
+  qexists_tac ‘n+99’
+  qexists_tac ‘1’
+  full_simp_tac bool_ss [steps_def]
+  full_simp_tac pure_ss []
 QED
 
 (*EVAL “semantics (Val (SNum 3))”*)
